

**SANTA CLARA UNIVERSITY**  
***Electrical Engineering Department***

*Homework 1*

2.1. The proof is as follows:

$$\begin{aligned}(x + y) \cdot (x + z) &= xx + xz + xy + yz \\&= x + xz + xy + yz \\&= x(1 + z + y) + yz \\&= x \cdot 1 + yz \\&= x + yz\end{aligned}$$

2.2. The proof is as follows:

$$\begin{aligned}(x + y) \cdot (x + \bar{y}) &= xx + xy + x\bar{y} + y\bar{y} \\&= x + xy + x\bar{y} + 0 \\&= x(1 + y + \bar{y}) \\&= x \cdot 1 \\&= x\end{aligned}$$

2.3. Manipulate the left hand side as follows:

$$\begin{aligned}xy + yz + \bar{x}z &= xy + (x + \bar{x})yz + \bar{x}z \\&= xy + xyz + \bar{x}yz + \bar{x}z \\&= xy(1 + z) + \bar{x}(y + 1)z \\&= xy \cdot 1 + \bar{x} \cdot 1 \cdot z \\&= xy + \bar{x}z\end{aligned}$$

2.10. Starting with the canonical sum-of-products for  $f$  get

$$\begin{aligned}f &= \bar{x}_1\bar{x}_2x_3 + \bar{x}_1x_2\bar{x}_3 + \bar{x}_1x_2x_3 + x_1\bar{x}_2\bar{x}_3 + x_1\bar{x}_2x_3 + x_1x_2\bar{x}_3 + x_1x_2x_3 \\&= x_1(\bar{x}_2\bar{x}_3 + \bar{x}_2x_3 + x_2\bar{x}_3 + x_2x_3) + x_2(\bar{x}_1\bar{x}_3 + \bar{x}_1x_3 + x_1\bar{x}_3 + x_1x_3) \\&\quad + x_3(\bar{x}_1\bar{x}_2 + \bar{x}_1x_2 + x_1\bar{x}_2 + x_1x_2) \\&= x_1(\bar{x}_2(\bar{x}_3 + x_3) + x_2(\bar{x}_3 + x_3)) + x_2(\bar{x}_1(\bar{x}_3 + x_3) + x_1(\bar{x}_3 + x_3)) \\&\quad + x_3(\bar{x}_1(\bar{x}_2 + x_2) + x_1(\bar{x}_2 + x_2)) \\&= x_1(\bar{x}_2 \cdot 1 + x_2 \cdot 1) + x_2(\bar{x}_1 \cdot 1 + x_1 \cdot 1) + x_3(\bar{x}_1 \cdot 1 + x_1 \cdot 1) \\&= x_1(\bar{x}_2 + x_2) + x_2(\bar{x}_1 + x_1) + x_3(\bar{x}_1 + x_1) \\&= x_1 \cdot 1 + x_2 \cdot 1 + x_3 \cdot 1 \\&= x_1 + x_2 + x_3\end{aligned}$$

2.11. Starting with the canonical product-of-sums for  $f$  can derive:

$$\begin{aligned}
 f &= (x_1 + x_2 + x_3)(x_1 + x_2 + \bar{x}_3)(x_1 + \bar{x}_2 + x_3)(x_1 + \bar{x}_2 + \bar{x}_3) \cdot \\
 &\quad (\bar{x}_1 + x_2 + x_3)(\bar{x}_1 + x_2 + \bar{x}_3)(\bar{x}_1 + \bar{x}_2 + x_3) \\
 &= ((x_1 + x_2 + x_3)(x_1 + x_2 + \bar{x}_3))((x_1 + \bar{x}_2 + x_3)(x_1 + \bar{x}_2 + \bar{x}_3)) \cdot \\
 &\quad ((\bar{x}_1 + x_2 + x_3)(\bar{x}_1 + x_2 + \bar{x}_3))((\bar{x}_1 + \bar{x}_2 + x_3)(\bar{x}_1 + \bar{x}_2 + \bar{x}_3)) \\
 &= (x_1 + x_2 + x_3\bar{x}_3)(x_1 + \bar{x}_2 + x_3\bar{x}_3) \cdot \\
 &\quad (\bar{x}_1 + x_2 + x_3\bar{x}_3)(\bar{x}_1 + \bar{x}_2 + x_3) \\
 &= (x_1 + x_2)(x_1 + \bar{x}_2)(\bar{x}_1 + x_2)(\bar{x}_1 + x_3) \\
 &= (x_1 + x_2\bar{x}_2)(\bar{x}_1 + x_2x_3) \\
 &= x_1(\bar{x}_1 + x_2x_3) \\
 &= x_1\bar{x}_1 + x_1x_2x_3 \\
 &= x_1x_2x_3
 \end{aligned}$$

2.25. The simplest SOP expression for the function is

$$\begin{aligned}
 f &= \bar{x}_1\bar{x}_3\bar{x}_5 + \bar{x}_1\bar{x}_3\bar{x}_4 + \bar{x}_1x_4x_5 + x_1\bar{x}_2\bar{x}_3x_5 \\
 &= \bar{x}_1\bar{x}_3\bar{x}_5 + \bar{x}_1\bar{x}_3\bar{x}_4 + \bar{x}_1x_4x_5 + \bar{x}_1\bar{x}_3x_5 + x_1\bar{x}_2\bar{x}_3x_5 \\
 &= \bar{x}_1\bar{x}_3 + \bar{x}_1\bar{x}_3\bar{x}_4 + \bar{x}_1x_4x_5 + x_1\bar{x}_2\bar{x}_3x_5 \\
 &= \bar{x}_1\bar{x}_3 + \bar{x}_1x_4x_5 + x_1\bar{x}_2\bar{x}_3x_5 \\
 &= \bar{x}_1\bar{x}_3 + \bar{x}_1x_4x_5 + \bar{x}_2\bar{x}_3x_5
 \end{aligned}$$

2.26. The simplest POS expression for the function is

$$\begin{aligned}
 f &= (\bar{x}_1 + \bar{x}_3 + \bar{x}_4)(\bar{x}_2 + \bar{x}_3 + x_4)(x_1 + \bar{x}_2 + \bar{x}_3) \\
 &= (\bar{x}_1 + \bar{x}_3 + \bar{x}_4)(\bar{x}_2 + \bar{x}_3 + x_4)(\bar{x}_1 + \bar{x}_2 + \bar{x}_3)(x_1 + \bar{x}_2 + \bar{x}_3) \\
 &= (\bar{x}_1 + \bar{x}_3 + \bar{x}_4)(\bar{x}_2 + \bar{x}_3 + x_4)(\bar{x}_2 + \bar{x}_3) \\
 &= (\bar{x}_1 + \bar{x}_3 + \bar{x}_4)(\bar{x}_2 + \bar{x}_3)
 \end{aligned}$$